coq/main.v
@@ -1,5 +1,0 @@
-Require Import MutualDistrust.rfj.
-
-(* Theorem: Structured full abstraction for the structured context
-   languages defined by RFJ and the target machine implies mutual
-   distrust for RFJ and the target machine. *)
